SpecDevice simplified

SpecDevice.v
@@ -34,30 +34,84 @@ Local Open Scope guru_scope.
 Definition regBits (lgRegBytes : nat) : Z :=
   NatZ_mul (Nat.pow 2 lgRegBytes) 8.
 
-Inductive RegionKind (regionSize : nat) (hasTags : bool) :=
-| InternalMem (init : option (option (type (Array regionSize (Bit 8)))))
-| ExternalMem (numDXlen : nat)
-| RegisterMem (lgRegBytes : nat)
-              (regs : list (string * option (type (Bit (regBits lgRegBytes)))))
-              (pfSize : Is_true (regionSize =? (length regs * Nat.pow 2 lgRegBytes))%nat)
-              (pfRegAligned : Is_true (if hasTags then (Nat.pow 2 lgRegBytes mod DXlenBytes =? 0)%nat else true)).
+Definition LgDXlenBytes : nat := Eval compute in Z.to_nat LgNumBytesFullCapSz.
 
-Arguments InternalMem [regionSize hasTags] init.
-Arguments ExternalMem [regionSize hasTags] numDXlen.
-Arguments RegisterMem [regionSize hasTags] lgRegBytes regs pfSize pfRegAligned.
+Inductive LineConfig :=
+| TaggedLine (lgLineBytes : nat) (pf : Is_true (LgDXlenBytes <=? lgLineBytes)%nat)
+| RawLine    (lgLineBytes : nat).
+
+Definition cfgHasTags (cfg : LineConfig) : bool :=
+  match cfg with
+  | TaggedLine _ _ => true
+  | RawLine _ => false
+  end.
+
+Definition cfgLgLineBytes (cfg : LineConfig) : nat :=
+  match cfg with
+  | TaggedLine lgBytes _ => lgBytes
+  | RawLine lgBytes => lgBytes
+  end.
+
+Definition cfgLineBytes (cfg : LineConfig) : nat :=
+  Nat.pow 2 (cfgLgLineBytes cfg).
+
+Definition cfgNumLineTags (cfg : LineConfig) : nat :=
+  match cfg with
+  | TaggedLine lgBytes _ => Nat.pow 2 (lgBytes - LgDXlenBytes)
+  | RawLine _ => 0%nat
+  end.
+
+Notation LineReadRp cfg := (STRUCT_TYPE {
+  "data" :: Array (cfgLineBytes cfg) (Bit 8) ;
+  "tag"  :: Array (cfgNumLineTags cfg) Bool
+}).
+
+Notation LineWriteRq cfg := (STRUCT_TYPE {
+  "addr"     :: Addr ;
+  "data"     :: Array (cfgLineBytes cfg) (Bit 8) ;
+  "dataMask" :: Array (cfgLineBytes cfg) Bool ;
+  "tag"      :: Array (cfgNumLineTags cfg) Bool ;
+  "tagMask"  :: Array (cfgNumLineTags cfg) Bool
+}).
+
+Inductive RegionKind (regionName : string) (regionSize : nat) (cfg : LineConfig) :=
+| InternalMem (init : option (option (type (Array regionSize (Bit 8)))))
+| ExternalMem
+| CustomMem (children : list (Tree Elem))
+            (readAction : forall ty, Expr ty Addr ->
+                          Action ty (Node regionName children) (LineReadRp cfg))
+            (writeAction : forall ty, Expr ty (LineWriteRq cfg) ->
+                           Action ty (Node regionName children) (Bit 0)).
+
+Arguments InternalMem {regionName regionSize cfg} init.
+Arguments ExternalMem {regionName regionSize cfg}.
+Arguments CustomMem {regionName regionSize cfg} children readAction writeAction.
 
 Record MemRegion := {
-  regionName       : string ;
-  regionBase       : Z ;
-  regionSize       : nat ;
-  hasTags          : bool ;
-  isReadOnly       : bool ;
-  regionKind       : RegionKind regionSize hasTags ;
-  regionInMemory   : Is_true ((0 <=? regionBase) && (regionBase + Z.of_nat regionSize <=? Z.shiftl 1 Xlen))%Z ;
-  regionAligned    : Is_true (if hasTags
-                              then (regionBase mod Z.of_nat DXlenBytes =? 0)%Z && (regionSize mod DXlenBytes =? 0)%nat
-                              else true)
+  regionName     : string ;
+  regionBase     : Z ;
+  regionSize     : nat ;
+  regionLineCfg  : LineConfig ;
+  isReadOnly     : bool ;
+  regionKind     : RegionKind regionName regionSize regionLineCfg ;
+  regionInMemory : Is_true ((0 <=? regionBase) && (regionBase + Z.of_nat regionSize <=? Z.shiftl 1 Xlen))%Z ;
+  regionAligned  : Is_true (
+    (regionBase mod (2 ^ Z.of_nat (cfgLgLineBytes regionLineCfg)) =? 0)%Z &&
+    (regionSize mod (cfgLineBytes regionLineCfg) =? 0)%nat
+  )
 }.
+
+Definition hasTags (r : MemRegion) : bool :=
+  cfgHasTags r.(regionLineCfg).
+
+Definition lgLineBytes (r : MemRegion) : nat :=
+  cfgLgLineBytes r.(regionLineCfg).
+
+Definition lineBytes (r : MemRegion) : nat :=
+  cfgLineBytes r.(regionLineCfg).
+
+Definition numLineTags (r : MemRegion) : nat :=
+  cfgNumLineTags r.(regionLineCfg).
 
 Definition disjointBool (r1 r2 : MemRegion) : bool :=
   (r1.(regionBase) + Z.of_nat r1.(regionSize) <=? r2.(regionBase))%Z ||
@@ -73,41 +127,31 @@ Definition isRegionAddr {ty : Kind -> Type} (r : MemRegion) (addr : Expr ty Addr
   And [ Sge addr $(r.(regionBase)) ; Slt addr $(r.(regionBase) + Z.of_nat r.(regionSize)) ].
 
 Definition regionTagSize (r : MemRegion) : nat :=
-  if r.(hasTags) then (r.(regionSize) / DXlenBytes)%nat else 0%nat.
+  if hasTags r then (r.(regionSize) / DXlenBytes)%nat else 0%nat.
 
 (* ===========================================================================
- * 2. External Transaction Payloads
+ * 2. Payload Utilities
  * =========================================================================== *)
-
-Definition ExternalMemWriteRq (numBytes : nat) := STRUCT_TYPE {
-  "addr" :: Addr ;
-  "data" :: Array numBytes (Bit 8) ;
-  "mask" :: Array numBytes Bool
-}.
-
-Definition ExternalTagWriteRq (numDXlen : nat) := STRUCT_TYPE {
-  "addr" :: Bit TagAddrWidth ;
-  "tag"  :: Array numDXlen Bool ;
-  "mask" :: Array numDXlen Bool
-}.
 
 Definition embedCapBytes {ty : Kind -> Type} (numBytes : nat)
   (capBytes : Expr ty (Array (Z.to_nat NumBytesFullCapSz) (Bit 8)))
   : Expr ty (Array numBytes (Bit 8)) :=
   ArrayBuilder (fun (i : FinType numBytes) =>
-    if (finNum i <? Z.to_nat NumBytesFullCapSz)%nat then
-      ReadArray capBytes (Const ty (Bit LgNumBytesFullCapSz) (bits.of_Z LgNumBytesFullCapSz (Z.of_nat (finNum i))))
-    else
-      Const ty (Bit 8) Zmod.zero).
+    readNatToFinType (Const ty (Bit 8) Zmod.zero)
+                     (ReadArrayConst capBytes)
+                     (finNum i)).
 
-Lemma add_sub_cancel (A L : Z) : (L + (A - L))%Z = A.
+Lemma add_sub_cancel (a l : Z) : (l + (a - l))%Z = a.
 Proof. lia. Qed.
 
 (* ===========================================================================
  * 3. Converting a MemRegion into a Tree
  * =========================================================================== *)
 
-Definition internalMemRegionChildren (r : MemRegion) (init : option (option (type (Array r.(regionSize) (Bit 8))))) : list (Tree Elem) :=
+Definition internalMemRegionChildren
+           (r : MemRegion)
+           (init : option (option (type (Array r.(regionSize) (Bit 8)))))
+           : list (Tree Elem) :=
   [ Leaf "mainMem" (EMem {| memSize := r.(regionSize);
                             memKind := Bit 8;
                             memPort := 1;
@@ -119,61 +163,37 @@ Definition internalMemRegionChildren (r : MemRegion) (init : option (option (typ
                                             (Is_true_Nat_eq_implies (repeat_length _ _)))) |})
   ].
 
-Definition externalMemRegionChildren (r : MemRegion) (numDXlen : nat) : list (Tree Elem) :=
-  let numBytes := (numDXlen * DXlenBytes)%nat in
-  [ Leaf "externalMemReadRq"  (ESend Addr) ;
-    Leaf "externalMemReadRp"  (ERecv (Array numBytes (Bit 8))) ;
-    Leaf "externalMemWriteRq" (ESend (ExternalMemWriteRq numBytes)) ;
-    Leaf "externalTagReadRq"  (ESend (Bit TagAddrWidth)) ;
-    Leaf "externalTagReadRp"  (ERecv (Array numDXlen Bool)) ;
-    Leaf "externalTagWriteRq" (ESend (ExternalTagWriteRq numDXlen))
-  ].
-
-Definition registerMemRegionChildren
-           (r : MemRegion)
-           (lgRegBytes : nat)
-           (regs : list (string * option (type (Bit (regBits lgRegBytes)))))
-           : list (Tree Elem) :=
-  [ Node "regs" (
-      map (fun '(name, initVal) =>
-        Leaf name (EReg (Build_Reg (Bit (regBits lgRegBytes)) initVal))
-      ) regs
-    ) ;
-    Leaf "tags" (EReg (Build_Reg (Array (regionTagSize r) Bool)
-                                 (Some (Build_SameTuple (tupleElems := List.repeat false (regionTagSize r))
-                                                        (Is_true_Nat_eq_implies (repeat_length _ _))))))
+Definition externalMemRegionChildren (r : MemRegion) : list (Tree Elem) :=
+  [ Leaf "lineReadRq" (ESend Addr) ;
+    Leaf "lineReadRp" (ERecv (LineReadRp r.(regionLineCfg))) ;
+    Leaf "lineWriteRq" (ESend (LineWriteRq r.(regionLineCfg)))
   ].
 
 Arguments internalMemRegionChildren r init : clear implicits.
-Arguments externalMemRegionChildren r numDXlen : clear implicits.
-Arguments registerMemRegionChildren r lgRegBytes regs : clear implicits.
+Arguments externalMemRegionChildren r : clear implicits.
 
 Definition internalMemRegionTree (r : MemRegion) (init : option (option (type (Array r.(regionSize) (Bit 8))))) : Tree Elem :=
   Node r.(regionName) (internalMemRegionChildren r init).
 
-Definition externalMemRegionTree (r : MemRegion) (numDXlen : nat) : Tree Elem :=
-  Node r.(regionName) (externalMemRegionChildren r numDXlen).
+Definition externalMemRegionTree (r : MemRegion) : Tree Elem :=
+  Node r.(regionName) (externalMemRegionChildren r).
 
-Definition registerMemRegionTree
-           (r : MemRegion)
-           (lgRegBytes : nat)
-           (regs : list (string * option (type (Bit (regBits lgRegBytes)))))
-           : Tree Elem :=
-  Node r.(regionName) (registerMemRegionChildren r lgRegBytes regs).
+Definition customMemRegionTree (r : MemRegion) (children : list (Tree Elem)) : Tree Elem :=
+  Node r.(regionName) children.
 
 Arguments internalMemRegionTree r init : clear implicits.
-Arguments externalMemRegionTree r numDXlen : clear implicits.
-Arguments registerMemRegionTree r lgRegBytes regs : clear implicits.
+Arguments externalMemRegionTree r : clear implicits.
+Arguments customMemRegionTree r children : clear implicits.
 
 Definition memRegionTree (r : MemRegion) : Tree Elem :=
   match r.(regionKind) with
   | InternalMem init => internalMemRegionTree r init
-  | ExternalMem numDXlen => externalMemRegionTree r numDXlen
-  | RegisterMem lg regs _ _ => registerMemRegionTree r lg regs
+  | ExternalMem => externalMemRegionTree r
+  | CustomMem children _ _ => customMemRegionTree r children
   end.
 
 (* ===========================================================================
- * 4. Generic Multi-Byte Read & Write for a MemRegion
+ * 4. Line-Level Actions for Each Region Kind
  * =========================================================================== *)
 
 Section InternalMemRegionActions.
@@ -182,51 +202,40 @@ Section InternalMemRegionActions.
   Variable ty : Kind -> Type.
 
   Local Definition tInt := internalMemRegionTree r init.
-
   Local Definition mainMemPath : MemPath tInt := getChildMemPathTree tInt "mainMem".
   Local Definition tagsPath : MemPath tInt := getChildMemPathTree tInt "tags".
 
-  Definition internalMemRegionRead (addr : Expr ty Addr) : Action ty tInt FullCapWithTag :=
+  Definition internalMemRegionLineRead (addr : Expr ty Addr)
+             : Action ty tInt (LineReadRp r.(regionLineCfg)) :=
     Let offset <- getMemOffset r.(regionBase) (Z.of_nat r.(regionSize)) addr ;
-    Let tagAddr : Bit TagAddrWidth <- TruncMsb TagAddrWidth LgNumBytesFullCapSz addr ;
-    Let tagOffset <- getMemOffset (Z.shiftr r.(regionBase) LgNumBytesFullCapSz) (Z.of_nat (regionTagSize r)) #tagAddr ;
-    LetA dataBytes : Array (Z.to_nat NumBytesFullCapSz) (Bit 8) <-
-      sliceMem mainMemPath I (Z.to_nat NumBytesFullCapSz) #offset ;
-    Let rawData : Bit FullCapSz <- ToBit #dataBytes ;
-    LetA tagArr : Array 1 Bool <-
-      if r.(hasTags) then
-        sliceMem tagsPath I 1 #tagOffset
-      else
-        Return ConstDef ;
-    Let rawTag : Bool <- ReadArrayConst #tagArr (@Build_FinType 1 0 I) ;
-    Let res : FullCapWithTag <- STRUCT {
-      "tag"  ::= #rawTag ;
-      "cap"  ::= FromBit Cap (TruncMsb Xlen Xlen #rawData) ;
-      "addr" ::= TruncLsb Xlen Xlen #rawData
-    } ;
-    Return #res.
+    LetA dataBytes : Array (lineBytes r) (Bit 8) <-
+      sliceMem mainMemPath I (lineBytes r) #offset ;
+    LetA tagArr : Array (numLineTags r) Bool <-
+      if hasTags r then (
+        Let tagAddr : Bit TagAddrWidth <- TruncMsb TagAddrWidth LgNumBytesFullCapSz addr ;
+        Let tagOffset <- getMemOffset (Z.shiftr r.(regionBase) LgNumBytesFullCapSz) (Z.of_nat (regionTagSize r)) #tagAddr ;
+        sliceMem tagsPath I (numLineTags r) #tagOffset
+      ) else (
+        Return ConstDef
+      ) ;
+    @Return ty tInt (LineReadRp r.(regionLineCfg)) (STRUCT {
+      "data" ::= #dataBytes ;
+      "tag"  ::= #tagArr
+    }).
 
-  Definition internalMemRegionWrite
-             (addr : Expr ty Addr)
-             (stVal : Expr ty FullCapWithTag)
-             (memSize : Expr ty (Bit LgLgNumBytesFullCapSz))
+  Definition internalMemRegionLineWrite
+             (rq : Expr ty (LineWriteRq r.(regionLineCfg)))
              : Action ty tInt (Bit 0) :=
     if r.(isReadOnly) then (
       Retv
     ) else (
-      Let offset <- getMemOffset r.(regionBase) (Z.of_nat r.(regionSize)) addr ;
-      Let tagAddr : Bit TagAddrWidth <- TruncMsb TagAddrWidth LgNumBytesFullCapSz addr ;
-      Let tagOffset <- getMemOffset (Z.shiftr r.(regionBase) LgNumBytesFullCapSz) (Z.of_nat (regionTagSize r)) #tagAddr ;
-      Let isCap : Bool <- Eq memSize $LgNumBytesFullCapSz ;
-      Let rawData : Bit FullCapSz <-
-        ITE #isCap
-            {< ToBit (stVal`"cap"), stVal`"addr" >}
-            (ZeroExtendTo FullCapSz (stVal`"addr")) ;
-      Let num_bytes : Bit (LgNumBytesFullCapSz + 1) <- Sll $1 memSize ;
-      Let byteMask : Array (Z.to_nat NumBytesFullCapSz) Bool <- Not (invMask (Z.to_nat NumBytesFullCapSz) #num_bytes) ;
-      Act (updSliceMem mainMemPath (Z.to_nat NumBytesFullCapSz) #offset (FromBit (Array (Z.to_nat NumBytesFullCapSz) (Bit 8)) #rawData) #byteMask) ;
-      if r.(hasTags) then (
-        WriteMem tagsPath #tagOffset (stVal`"tag") Retv
+      Let offset <- getMemOffset r.(regionBase) (Z.of_nat r.(regionSize)) (rq`"addr") ;
+      Act (updSliceMem mainMemPath (lineBytes r) #offset (rq`"data") (rq`"dataMask")) ;
+      if hasTags r then (
+        Let tagAddr : Bit TagAddrWidth <- TruncMsb TagAddrWidth LgNumBytesFullCapSz (rq`"addr") ;
+        Let tagOffset <- getMemOffset (Z.shiftr r.(regionBase) LgNumBytesFullCapSz) (Z.of_nat (regionTagSize r)) #tagAddr ;
+        Act (updSliceMem tagsPath (numLineTags r) #tagOffset (rq`"tag") (rq`"tagMask")) ;
+        Retv
       ) else (
         Retv
       )
@@ -234,346 +243,271 @@ Section InternalMemRegionActions.
 
 End InternalMemRegionActions.
 
-Arguments internalMemRegionRead r init [ty] addr.
-Arguments internalMemRegionWrite r init [ty] addr stVal memSize.
+Arguments internalMemRegionLineRead r init [ty] addr.
+Arguments internalMemRegionLineWrite r init [ty] rq.
 
 Section ExternalMemRegionActions.
   Variable r : MemRegion.
-  Variable numDXlen : nat.
   Variable ty : Kind -> Type.
 
-  Local Definition tExt := externalMemRegionTree r numDXlen.
-  Local Definition numBytes := (numDXlen * DXlenBytes)%nat.
-  Local Definition lgNumDXlen := Z.log2_up (Z.of_nat numDXlen).
-  Local Definition lgLineBytes := (LgNumBytesFullCapSz + lgNumDXlen)%Z.
+  Local Definition tExt := externalMemRegionTree r.
+  Local Definition pLineReadRq : SendPath tExt := getChildSendPathTree tExt "lineReadRq".
+  Local Definition pLineReadRp : RecvPath tExt := getChildRecvPathTree tExt "lineReadRp".
+  Local Definition pLineWriteRq : SendPath tExt := getChildSendPathTree tExt "lineWriteRq".
 
-  Local Definition castAddr (addr : Expr ty Addr) : Expr ty (Bit ((lgLineBytes + (AddrSz - lgLineBytes))%Z)) :=
-    castBits (eq_sym (add_sub_cancel AddrSz lgLineBytes)) addr.
+  Definition externalMemRegionLineRead (addr : Expr ty Addr)
+             : Action ty tExt (LineReadRp r.(regionLineCfg)) :=
+    Send pLineReadRq addr (
+    Recv "rp" pLineReadRp (fun rp =>
+    Return #rp)).
 
-  Local Definition lineOffset (addr : Expr ty Addr) : Expr ty (Bit lgLineBytes) :=
-    TruncLsb (AddrSz - lgLineBytes)%Z lgLineBytes (castAddr addr).
-
-  Local Definition lineIndex (addr : Expr ty Addr) : Expr ty (Bit (AddrSz - lgLineBytes)%Z) :=
-    TruncMsb (AddrSz - lgLineBytes)%Z lgLineBytes (castAddr addr).
-
-  Local Definition lineAddr (addr : Expr ty Addr) : Expr ty Addr :=
-    castBits (add_sub_cancel AddrSz lgLineBytes) {< lineIndex addr, Const ty (Bit lgLineBytes) Zmod.zero >}.
-
-  Local Definition nextLineAddr (addr : Expr ty Addr) : Expr ty Addr :=
-    castBits (add_sub_cancel AddrSz lgLineBytes) {< Add [ lineIndex addr ; Const ty (Bit (AddrSz - lgLineBytes)%Z) (Zmod.of_Z _ 1) ], Const ty (Bit lgLineBytes) Zmod.zero >}.
-
-  Local Definition lineTagAddr (addr : Expr ty Addr) : Expr ty (Bit TagAddrWidth) :=
-    TruncMsb TagAddrWidth LgNumBytesFullCapSz (lineAddr addr).
-
-  Local Definition add1 (addr : Expr ty Addr) : Expr ty (Array numBytes Bool) :=
-    FromBit (Array numBytes Bool)
-      (Not (Sll (ConstBit (InvDefault _)) (lineOffset addr))).
-
-  Local Definition pMemReadRq : SendPath tExt := getChildSendPathTree tExt "externalMemReadRq".
-  Local Definition pMemReadRp : RecvPath tExt := getChildRecvPathTree tExt "externalMemReadRp".
-  Local Definition pMemWriteRq : SendPath tExt := getChildSendPathTree tExt "externalMemWriteRq".
-  Local Definition pTagReadRq : SendPath tExt := getChildSendPathTree tExt "externalTagReadRq".
-  Local Definition pTagReadRp : RecvPath tExt := getChildRecvPathTree tExt "externalTagReadRp".
-  Local Definition pTagWriteRq : SendPath tExt := getChildSendPathTree tExt "externalTagWriteRq".
-
-  Definition externalMemRegionRead
-             (addr : Expr ty Addr)
-             (memSize : Expr ty (Bit LgLgNumBytesFullCapSz))
-             : Action ty tExt FullCapWithTag :=
-    Let numBytesActive : Bit (lgLineBytes + 1)%Z <-
-                           Sll (Const ty (Bit (lgLineBytes + 1)%Z) (bits.of_Z _ 1))
-                             (ZeroExtend (lgLineBytes + 1 - LgLgNumBytesFullCapSz)%Z memSize) ;
-    Let endOffset : Bit (lgLineBytes + 1)%Z <-
-      Add [ ZeroExtend 1 (lineOffset addr) ; #numBytesActive ] ;
-    Let crosses : Bool <- FromBit Bool (TruncMsb 1 lgLineBytes #endOffset) ;
-    Send pMemReadRq (lineAddr addr) (
-    Recv "lineData1" pMemReadRp (fun lineData1 =>
-    LetIf lineDataMerged : Array numBytes (Bit 8) <-
-      If #crosses Then (
-        Send pMemReadRq (nextLineAddr addr) (
-        Recv "lineData2" pMemReadRp (fun lineData2 =>
-        Return (ArrayBuilder (fun (i : FinType numBytes) =>
-          ITE (ReadArrayConst (add1 addr) i)
-              (ReadArrayConst #lineData2 i)
-              (ReadArrayConst #lineData1 i)))))
-      ) Else (
-        Return #lineData1
-      ) ;
-    Let rotData : Array numBytes (Bit 8) <- ArrayRotr 8 #lineDataMerged (lineOffset addr) ;
-    Let capBytes : Array (Z.to_nat NumBytesFullCapSz) (Bit 8) <-
-      slice #rotData (Const ty (Bit 0) Zmod.zero) (Z.to_nat NumBytesFullCapSz) ;
-    Let rawData : Bit FullCapSz <- ToBit #capBytes ;
-    LetA rawTag : Bool <-
-      if r.(hasTags) then (
-        Send pTagReadRq (lineTagAddr addr) (
-        Recv "lineTags1" pTagReadRp (fun lineTags1 =>
-        Let isAligned : Bool <- Eq (lineOffset addr) (Const ty (Bit lgLineBytes) Zmod.zero) ;
-        Let isCap : Bool <- Eq memSize $LgNumBytesFullCapSz ;
-        Let tagSlot : Bit lgNumDXlen <- TruncMsb lgNumDXlen LgNumBytesFullCapSz (lineOffset addr) ;
-        Return (And [ #isAligned ; #isCap ; ReadArray #lineTags1 #tagSlot ])))
-      ) else (
-        Return (ConstBool false)
-      ) ;
-    Let res : FullCapWithTag <- STRUCT {
-      "tag"  ::= #rawTag ;
-      "cap"  ::= FromBit Cap (TruncMsb Xlen Xlen #rawData) ;
-      "addr" ::= TruncLsb Xlen Xlen #rawData
-    } ;
-    Return #res)).
-
-  Definition externalMemRegionWrite
-             (addr : Expr ty Addr)
-             (stVal : Expr ty FullCapWithTag)
-             (memSize : Expr ty (Bit LgLgNumBytesFullCapSz))
+  Definition externalMemRegionLineWrite
+             (rq : Expr ty (LineWriteRq r.(regionLineCfg)))
              : Action ty tExt (Bit 0) :=
     if r.(isReadOnly) then (
       Retv
     ) else (
-      Let isCap : Bool <- Eq memSize $LgNumBytesFullCapSz ;
+      Send pLineWriteRq rq Retv
+    ).
+
+End ExternalMemRegionActions.
+
+Arguments externalMemRegionLineRead r [ty] addr.
+Arguments externalMemRegionLineWrite r [ty] rq.
+
+Section CustomMemRegionActions.
+  Variable r : MemRegion.
+  Variable children : list (Tree Elem).
+  Variable readAction : forall ty, Expr ty Addr ->
+                        Action ty (Node r.(regionName) children)
+                               (LineReadRp r.(regionLineCfg)).
+  Variable writeAction : forall ty, Expr ty (LineWriteRq r.(regionLineCfg)) ->
+                         Action ty (Node r.(regionName) children) (Bit 0).
+  Variable ty : Kind -> Type.
+
+  Local Definition tCust := customMemRegionTree r children.
+
+  Definition customMemRegionLineRead (addr : Expr ty Addr)
+             : Action ty tCust (LineReadRp r.(regionLineCfg)) :=
+    readAction addr.
+
+  Definition customMemRegionLineWrite
+             (rq : Expr ty (LineWriteRq r.(regionLineCfg)))
+             : Action ty tCust (Bit 0) :=
+    if r.(isReadOnly) then (
+      Retv
+    ) else (
+      writeAction rq
+    ).
+
+End CustomMemRegionActions.
+
+Arguments customMemRegionLineRead r children readAction [ty] addr.
+Arguments customMemRegionLineWrite r children writeAction [ty] rq.
+
+Definition memRegionLineRead
+           {ty : Kind -> Type}
+           (r : MemRegion)
+           (addr : Expr ty Addr)
+           : Action ty (memRegionTree r) (LineReadRp r.(regionLineCfg)) :=
+  match r.(regionKind) as k return Action ty (match k with
+                                              | InternalMem init => internalMemRegionTree r init
+                                              | ExternalMem => externalMemRegionTree r
+                                              | CustomMem children _ _ => customMemRegionTree r children
+                                              end) (LineReadRp r.(regionLineCfg)) with
+  | InternalMem init => internalMemRegionLineRead r init addr
+  | ExternalMem => externalMemRegionLineRead r addr
+  | CustomMem children readAct writeAct => customMemRegionLineRead r children readAct addr
+  end.
+
+Definition memRegionLineWrite
+           {ty : Kind -> Type}
+           (r : MemRegion)
+           (rq : Expr ty (LineWriteRq r.(regionLineCfg)))
+           : Action ty (memRegionTree r) (Bit 0) :=
+  match r.(regionKind) as k return Action ty (match k with
+                                              | InternalMem init => internalMemRegionTree r init
+                                              | ExternalMem => externalMemRegionTree r
+                                              | CustomMem children _ _ => customMemRegionTree r children
+                                              end) (Bit 0) with
+  | InternalMem init => internalMemRegionLineWrite r init rq
+  | ExternalMem => externalMemRegionLineWrite r rq
+  | CustomMem children readAct writeAct => customMemRegionLineWrite r children writeAct rq
+  end.
+
+Arguments memRegionLineRead [ty] r addr.
+Arguments memRegionLineWrite [ty] r rq.
+
+(* ===========================================================================
+ * 5. Universal CHERI Capability Multi-Byte Read & Write for a MemRegion
+ * =========================================================================== *)
+
+Section MemRegionActions.
+  Variable r : MemRegion.
+  Variable ty : Kind -> Type.
+
+  Local Definition tR := memRegionTree r.
+  Local Definition lBytes := lineBytes r.
+  Local Definition nTags := numLineTags r.
+  Local Definition lgLineBytesZ := Z.of_nat (lgLineBytes r).
+
+  Local Definition castAddr (addr : Expr ty Addr) : Expr ty (Bit ((lgLineBytesZ + (AddrSz - lgLineBytesZ))%Z)) :=
+    castBits (eq_sym (add_sub_cancel AddrSz lgLineBytesZ)) addr.
+
+  Local Definition lineOffset (addr : Expr ty Addr) : Expr ty (Bit lgLineBytesZ) :=
+    TruncLsb (AddrSz - lgLineBytesZ)%Z lgLineBytesZ (castAddr addr).
+
+  Local Definition lineIndex (addr : Expr ty Addr) : Expr ty (Bit (AddrSz - lgLineBytesZ)%Z) :=
+    TruncMsb (AddrSz - lgLineBytesZ)%Z lgLineBytesZ (castAddr addr).
+
+  Local Definition lineAddr (addr : Expr ty Addr) : Expr ty Addr :=
+    castBits (add_sub_cancel AddrSz lgLineBytesZ) {< lineIndex addr, Const ty (Bit lgLineBytesZ) Zmod.zero >}.
+
+  Local Definition nextLineAddr (addr : Expr ty Addr) : Expr ty Addr :=
+    castBits (add_sub_cancel AddrSz lgLineBytesZ) {< Add [ lineIndex addr ; Const ty (Bit (AddrSz - lgLineBytesZ)%Z) (Zmod.of_Z _ 1) ], Const ty (Bit lgLineBytesZ) Zmod.zero >}.
+
+  Local Definition add1 (addr : Expr ty Addr) : Expr ty (Array lBytes Bool) :=
+    FromBit (Array lBytes Bool)
+      (Not (Sll (ConstBit (InvDefault _)) (lineOffset addr))).
+
+  Local Definition lgNumDXlenZ : Z := (lgLineBytesZ - LgNumBytesFullCapSz)%Z.
+
+  Local Definition castLineOffsetForTag (offset : Expr ty (Bit lgLineBytesZ))
+    : Expr ty (Bit (LgNumBytesFullCapSz + lgNumDXlenZ)%Z) :=
+    castBits (eq_sym (add_sub_cancel lgLineBytesZ LgNumBytesFullCapSz)) offset.
+
+  Local Definition tagSlot (addr : Expr ty Addr) : Expr ty (Bit lgNumDXlenZ) :=
+    TruncMsb lgNumDXlenZ LgNumBytesFullCapSz (castLineOffsetForTag (lineOffset addr)).
+
+  Definition memRegionRead
+             (addr : Expr ty Addr)
+             (memSize : Expr ty (Bit LgLgNumBytesFullCapSz))
+             : Action ty tR FullCapWithTag :=
+    Let capOffset : Bit LgNumBytesFullCapSz <- TruncLsb TagAddrWidth LgNumBytesFullCapSz addr ;
+    Let isCapAligned : Bool <- isZero #capOffset ;
+    Let isCap : Bool <- And [Eq memSize $LgNumBytesFullCapSz ; #isCapAligned] ;
+    Let numBytesActive : Bit (lgLineBytesZ + 1)%Z <-
+                           Sll (Const ty (Bit (lgLineBytesZ + 1)%Z) (bits.of_Z _ 1))
+                             (ZeroExtend (lgLineBytesZ + 1 - LgLgNumBytesFullCapSz)%Z memSize) ;
+    Let endOffset : Bit (lgLineBytesZ + 1)%Z <-
+      Add [ ZeroExtend 1 (lineOffset addr) ; #numBytesActive ] ;
+    Let crossesLine : Bool <- FromBit Bool (TruncMsb 1 lgLineBytesZ #endOffset) ;
+    LetA rp1 : LineReadRp r.(regionLineCfg) <- memRegionLineRead r (lineAddr addr) ;
+    LetIf lineDataMerged : Array lBytes (Bit 8) <-
+      If #crossesLine Then (
+        LetA rp2 : LineReadRp r.(regionLineCfg) <- memRegionLineRead r (nextLineAddr addr) ;
+        Return (ArrayBuilder (fun (i : FinType lBytes) =>
+          ITE (ReadArrayConst (add1 addr) i)
+              (ReadArrayConst (##rp2`"data") i)
+              (ReadArrayConst (##rp1`"data") i)))
+      ) Else (
+        Return (##rp1`"data")
+      ) ;
+    Let rotData : Array lBytes (Bit 8) <- ArrayRotr 8 #lineDataMerged (lineOffset addr) ;
+    Let dataBytes : Array (Z.to_nat NumBytesFullCapSz) (Bit 8) <-
+      slice #rotData (Const ty (Bit 0) Zmod.zero) (Z.to_nat NumBytesFullCapSz) ;
+    Let rawData : Bit FullCapSz <- ToBit #dataBytes ;
+    LetA rawTag : Bool <-
+      if hasTags r then (
+        Return (ReadArray (##rp1`"tag") (tagSlot addr))
+      ) else (
+        Return (ConstBool false)
+      ) ;
+    Let res : FullCapWithTag <- STRUCT {
+      "tag"  ::= And [ #isCap ; #rawTag ] ;
+      "cap"  ::= FromBit Cap (TruncMsb Xlen Xlen #rawData) ;
+      "addr" ::= TruncLsb Xlen Xlen #rawData
+    } ;
+    Return #res.
+
+  Definition memRegionWrite
+             (addr : Expr ty Addr)
+             (stVal : Expr ty FullCapWithTag)
+             (memSize : Expr ty (Bit LgLgNumBytesFullCapSz))
+             : Action ty tR (Bit 0) :=
+    if r.(isReadOnly) then (
+      Retv
+    ) else (
+      Let capOffset : Bit LgNumBytesFullCapSz <- TruncLsb TagAddrWidth LgNumBytesFullCapSz addr ;
+      Let isCapAligned : Bool <- isZero #capOffset ;
+      Let isCap : Bool <- And [Eq memSize $LgNumBytesFullCapSz ; #isCapAligned] ;
       Let rawData : Bit FullCapSz <-
         ITE #isCap
             {< ToBit (stVal`"cap"), stVal`"addr" >}
             (ZeroExtendTo FullCapSz (stVal`"addr")) ;
       Let capBytes : Array (Z.to_nat NumBytesFullCapSz) (Bit 8) <-
         FromBit (Array (Z.to_nat NumBytesFullCapSz) (Bit 8)) #rawData ;
-      Let baseData : Array numBytes (Bit 8) <- embedCapBytes numBytes #capBytes ;
-      Let rotData : Array numBytes (Bit 8) <- ArrayRotl 8 #baseData (lineOffset addr) ;
-      Let numBytesActive : Bit (lgLineBytes + 1)%Z <-
-                             Sll (Const ty (Bit (lgLineBytes + 1)%Z) (bits.of_Z _ 1))
-                               (ZeroExtend (lgLineBytes + 1 - LgLgNumBytesFullCapSz)%Z memSize) ;
-      Let endOffset : Bit (lgLineBytes + 1)%Z <-
+      Let baseData : Array lBytes (Bit 8) <- embedCapBytes lBytes #capBytes ;
+      Let rotData : Array lBytes (Bit 8) <- ArrayRotl 8 #baseData (lineOffset addr) ;
+      Let numBytesActive : Bit (lgLineBytesZ + 1)%Z <-
+                             Sll (Const ty (Bit (lgLineBytesZ + 1)%Z) (bits.of_Z _ 1))
+                               (ZeroExtend (lgLineBytesZ + 1 - LgLgNumBytesFullCapSz)%Z memSize) ;
+      Let endOffset : Bit (lgLineBytesZ + 1)%Z <-
         Add [ ZeroExtend 1 (lineOffset addr) ; #numBytesActive ] ;
-      Let crosses : Bool <- FromBit Bool (TruncMsb 1 lgLineBytes #endOffset) ;
-      Let isWrites : Array numBytes Bool <-
-        FromBit (Array numBytes Bool)
+      Let crossesLine : Bool <- FromBit Bool (TruncMsb 1 lgLineBytesZ #endOffset) ;
+      Let numBytesActiveDXlen : Bit (LgNumBytesFullCapSz + 1)%Z <-
+                             Sll (Const ty (Bit (LgNumBytesFullCapSz + 1)%Z) (bits.of_Z _ 1))
+                               (ZeroExtend (LgNumBytesFullCapSz + 1 - LgLgNumBytesFullCapSz)%Z memSize) ;
+      Let endOffsetDXlen : Bit (LgNumBytesFullCapSz + 1)%Z <-
+        Add [ ZeroExtend 1 #capOffset ; #numBytesActiveDXlen ] ;
+      Let crossesDXlen : Bool <- FromBit Bool (TruncMsb 1 LgNumBytesFullCapSz #endOffsetDXlen) ;
+      Let isWrites : Array lBytes Bool <-
+        FromBit (Array lBytes Bool)
           (rotateLeft (Not (Sll (ConstBit (InvDefault _)) #numBytesActive)) (lineOffset addr)) ;
-      Let mask1 : Array numBytes Bool <-
-        ArrayBuilder (fun (i : FinType numBytes) =>
+      Let mask1 : Array lBytes Bool <-
+        ArrayBuilder (fun (i : FinType lBytes) =>
           And [ ReadArrayConst #isWrites i ; Not (ReadArrayConst (add1 addr) i) ]) ;
-      Send pMemWriteRq (STRUCT {
-        "addr" ::= lineAddr addr ;
-        "data" ::= #rotData ;
-        "mask" ::= #mask1
-      }) (
-      Act (
-        if r.(hasTags) then (
-          Let tagSlot : Bit lgNumDXlen <- TruncMsb lgNumDXlen LgNumBytesFullCapSz (lineOffset addr) ;
-          Let tagMask1 : Array numDXlen Bool <-
-            FromBit (Array numDXlen Bool)
-              (Sll (ConstT (Bit (NatZ_mul numDXlen 1)) Zmod.one) #tagSlot) ;
-          Let tagVal1 : Array numDXlen Bool <-
-            FromBit (Array numDXlen Bool)
-              (Sll (ITE0 (And [ #isCap ; stVal`"tag" ]) (ConstT (Bit (NatZ_mul numDXlen 1)) Zmod.one)) #tagSlot) ;
-          Send pTagWriteRq (STRUCT {
-            "addr" ::= lineTagAddr addr ;
-            "tag"  ::= #tagVal1 ;
-            "mask" ::= #tagMask1
-          }) Retv
+      Let tagData1 : Array nTags Bool <-
+        if hasTags r then (
+          UpdateArray ConstDef (tagSlot addr) (And [ #isCap ; stVal`"tag" ])
         ) else (
-          Retv
-        )) ;
-      If #crosses Then (
-        Let mask2 : Array numBytes Bool <-
-          ArrayBuilder (fun (i : FinType numBytes) =>
+          ConstDef
+        ) ;
+      Let crossWithinLine : Bool <- And [ #crossesDXlen ; Not #crossesLine ] ;
+      Let nextTagSlot : Bit lgNumDXlenZ <- Add [ tagSlot addr ; Const ty (Bit lgNumDXlenZ) (bits.of_Z _ 1) ] ;
+      Let tagMask1 : Array nTags Bool <-
+        if hasTags r then (
+          UpdateArray
+            (UpdateArray ConstDef (tagSlot addr) (ConstBool true))
+            #nextTagSlot
+            #crossWithinLine
+        ) else (
+          ConstDef
+        ) ;
+      Act (memRegionLineWrite r (STRUCT {
+        "addr"     ::= lineAddr addr ;
+        "data"     ::= #rotData ;
+        "dataMask" ::= #mask1 ;
+        "tag"      ::= #tagData1 ;
+        "tagMask"  ::= #tagMask1
+      })) ;
+      If #crossesLine Then (
+        Let mask2 : Array lBytes Bool <-
+          ArrayBuilder (fun (i : FinType lBytes) =>
             And [ ReadArrayConst #isWrites i ; ReadArrayConst (add1 addr) i ]) ;
-        Send pMemWriteRq (STRUCT {
-          "addr" ::= nextLineAddr addr ;
-          "data" ::= #rotData ;
-          "mask" ::= #mask2
-        }) Retv
-      ) ;
-      Retv)
-    ).
-
-End ExternalMemRegionActions.
-
-Arguments externalMemRegionRead r numDXlen [ty] addr memSize.
-Arguments externalMemRegionWrite r numDXlen [ty] addr stVal memSize.
-
-Section RegisterMemRegionActions.
-  Variable r : MemRegion.
-  Variable lgRegBytes : nat.
-  Variable regs : list (string * option (type (Bit (regBits lgRegBytes)))).
-  Variable ty : Kind -> Type.
-
-  Local Definition tReg := registerMemRegionTree r lgRegBytes regs.
-  Local Definition numRegBytes : nat := Nat.pow 2 lgRegBytes.
-  Local Definition regBitsVal : Z := regBits lgRegBytes.
-  Local Definition regPaths : list (RegOfKind (t:=tReg) (Bit regBitsVal)) :=
-    getTreeRegsOfKind (Bit regBitsVal) tReg.
-
-  Local Definition castToRegSum (e : Expr ty Addr) : Expr ty (Bit (Z.of_nat lgRegBytes + (AddrSz - Z.of_nat lgRegBytes))%Z) :=
-    castBits (eq_sym (add_sub_cancel AddrSz (Z.of_nat lgRegBytes))) e.
-
-  Local Definition castFromRegSum (e : Expr ty (Bit (Z.of_nat lgRegBytes + (AddrSz - Z.of_nat lgRegBytes))%Z)) : Expr ty Addr :=
-    castBits (add_sub_cancel AddrSz (Z.of_nat lgRegBytes)) e.
-
-  Local Definition byteOffset (offset : Expr ty Addr) : Expr ty (Bit (Z.of_nat lgRegBytes)) :=
-    TruncLsb (AddrSz - Z.of_nat lgRegBytes) (Z.of_nat lgRegBytes) (castToRegSum offset).
-
-  Local Definition regIdx (offset : Expr ty Addr) : Expr ty (Bit (AddrSz - Z.of_nat lgRegBytes)) :=
-    TruncMsb (AddrSz - Z.of_nat lgRegBytes) (Z.of_nat lgRegBytes) (castToRegSum offset).
-
-  Local Definition byteOffsetAddr (offset : Expr ty Addr) : Expr ty Addr :=
-    castFromRegSum (ZeroExtend (AddrSz - Z.of_nat lgRegBytes)%Z (byteOffset offset)).
-
-  Local Definition numBytesActive (memSize : Expr ty (Bit LgLgNumBytesFullCapSz)) : Expr ty Addr :=
-    Sll (Const ty Addr (bits.of_Z _ 1)) (ZeroExtend (AddrSz - LgLgNumBytesFullCapSz)%Z memSize).
-
-  Local Definition endOffset (offset : Expr ty Addr) (memSize : Expr ty (Bit LgLgNumBytesFullCapSz)) : Expr ty Addr :=
-    Add [ byteOffsetAddr offset ; numBytesActive memSize ].
-
-  Local Definition crosses (offset : Expr ty Addr) (memSize : Expr ty (Bit LgLgNumBytesFullCapSz)) : Expr ty Bool :=
-    Sgt (endOffset offset memSize) $(Z.of_nat numRegBytes).
-
-  Local Definition tagSlot (offset : Expr ty Addr) : Expr ty (Bit TagAddrWidth) :=
-    TruncMsb TagAddrWidth LgNumBytesFullCapSz offset.
-
-  Local Definition tagsRegPath : RegPath tReg := getChildRegPathTree tReg "tags".
-
-  Definition registerMemRegionRead
-             (addr : Expr ty Addr)
-             (memSize : Expr ty (Bit LgLgNumBytesFullCapSz))
-             : Action ty tReg FullCapWithTag :=
-    Let offset : Addr <- Sub addr $(r.(regionBase)) ;
-    Let isCross : Bool <- crosses #offset memSize ;
-    LetA regVal1 : Bit regBitsVal <- readRegsList regPaths (regIdx #offset) ;
-    LetIf regVal2 : Bit regBitsVal <-
-      If #isCross Then (
-        readRegsList regPaths (Add [ regIdx #offset ; Const ty (Bit (AddrSz - Z.of_nat lgRegBytes)%Z) (Zmod.of_Z _ 1) ])
-      ) Else (
-        Return (Const ty (Bit regBitsVal) Zmod.zero)
-      ) ;
-    Let bytes1 : Array numRegBytes (Bit 8) <- FromBit (Array numRegBytes (Bit 8)) #regVal1 ;
-    Let bytes2 : Array numRegBytes (Bit 8) <- FromBit (Array numRegBytes (Bit 8)) #regVal2 ;
-    Let capBytes : Array (Z.to_nat NumBytesFullCapSz) (Bit 8) <-
-      ArrayBuilder (fun (i : FinType (Z.to_nat NumBytesFullCapSz)) =>
-        let srcByte :=
-          Add [ byteOffsetAddr #offset ;
-                Const ty Addr (bits.of_Z _ (Z.of_nat (finNum i))) ] in
-        let inReg2 := Sge srcByte $(Z.of_nat numRegBytes) in
-        let idxInReg :=
-          TruncLsb (AddrSz - Z.of_nat lgRegBytes)%Z (Z.of_nat lgRegBytes) (castToRegSum srcByte) in
-        ITE inReg2
-            (ReadArray #bytes2 idxInReg)
-            (ReadArray #bytes1 idxInReg)) ;
-    LetA rawTag : Bool <-
-      if r.(hasTags) then (
-        ReadReg "allTags" tagsRegPath (fun allTags =>
-        Return (ReadArray #allTags (tagSlot #offset)))
-      ) else (
-        Return (Const ty Bool false)
-      ) ;
-    Let res : FullCapWithTag <- STRUCT {
-      "tag"  ::= #rawTag ;
-      "cap"  ::= FromBit Cap (TruncMsb (FullCapSz - Xlen) Xlen (ToBit #capBytes)) ;
-      "addr" ::= TruncLsb (FullCapSz - Xlen) Xlen (ToBit #capBytes)
-    } ;
-    Return #res.
-
-  Definition registerMemRegionWrite
-             (addr : Expr ty Addr)
-             (stVal : Expr ty FullCapWithTag)
-             (memSize : Expr ty (Bit LgLgNumBytesFullCapSz))
-             : Action ty tReg (Bit 0) :=
-    if r.(isReadOnly) then (
-      Retv
-    ) else (
-      Let offset : Addr <- Sub addr $(r.(regionBase)) ;
-      Let isCross : Bool <- crosses #offset memSize ;
-      Let isCap : Bool <- Eq memSize $LgNumBytesFullCapSz ;
-      Let rawData : Bit FullCapSz <-
-        ITE #isCap
-            {< ToBit (stVal`"cap"), stVal`"addr" >}
-            (ZeroExtendTo FullCapSz (stVal`"addr")) ;
-      Let writeBytes : Array (Z.to_nat NumBytesFullCapSz) (Bit 8) <-
-        FromBit (Array (Z.to_nat NumBytesFullCapSz) (Bit 8)) #rawData ;
-      Let numActive : Addr <- numBytesActive memSize ;
-      Let bOffset : Addr <- byteOffsetAddr #offset ;
-      LetA oldVal1 : Bit regBitsVal <- readRegsList regPaths (regIdx #offset) ;
-      Let oldBytes1 : Array numRegBytes (Bit 8) <- FromBit (Array numRegBytes (Bit 8)) #oldVal1 ;
-      Let newBytes1 : Array numRegBytes (Bit 8) <-
-        ArrayBuilder (fun (k : FinType numRegBytes) =>
-          let kVal := Const ty Addr (bits.of_Z _ (Z.of_nat (finNum k))) in
-          let active :=
-            And [ Sge kVal #bOffset ;
-                  Slt (Sub kVal #bOffset) #numActive ] in
-          let srcIdx :=
-            TruncLsb TagAddrWidth LgNumBytesFullCapSz (Sub kVal #bOffset) in
-          ITE active (ReadArray #writeBytes srcIdx) (ReadArrayConst #oldBytes1 k)) ;
-      Act (writeRegsList regPaths (regIdx #offset) (ToBit #newBytes1)) ;
-      If #isCross Then (
-        Let nextIdx : Bit (AddrSz - Z.of_nat lgRegBytes)%Z <-
-          Add [ regIdx #offset ; Const ty (Bit (AddrSz - Z.of_nat lgRegBytes)%Z) (Zmod.of_Z _ 1) ] ;
-        LetA oldVal2 : Bit regBitsVal <- readRegsList regPaths #nextIdx ;
-        Let oldBytes2 : Array numRegBytes (Bit 8) <- FromBit (Array numRegBytes (Bit 8)) #oldVal2 ;
-        Let newBytes2 : Array numRegBytes (Bit 8) <-
-          ArrayBuilder (fun (k : FinType numRegBytes) =>
-            let dist :=
-              Sub $(Z.of_nat numRegBytes + Z.of_nat (finNum k)) #bOffset in
-            let active := Slt dist #numActive in
-            let srcIdx := TruncLsb TagAddrWidth LgNumBytesFullCapSz dist in
-            ITE active (ReadArray #writeBytes srcIdx) (ReadArrayConst #oldBytes2 k)) ;
-        writeRegsList regPaths #nextIdx (ToBit #newBytes2)
-      ) ;
-      if r.(hasTags) then (
-        ReadReg "oldTags" tagsRegPath (fun oldTags =>
-        Let newTags : Array (regionTagSize r) Bool <-
-          ArrayBuilder (fun (s : FinType (regionTagSize r)) =>
-            let sVal := Const ty (Bit TagAddrWidth) (bits.of_Z _ (Z.of_nat (finNum s))) in
-            let isTargetSlot := Eq sVal (tagSlot #offset) in
-            let isNextSlot :=
-              And [ #isCross ;
-                    Eq sVal (Add [ tagSlot #offset ;
-                                   Const ty (Bit TagAddrWidth) (bits.of_Z _ 1) ]) ] in
-            ITE isTargetSlot
-                (ITE #isCap (stVal`"tag") (Const ty Bool false))
-                (ITE isNextSlot
-                     (Const ty Bool false)
-                     (ReadArrayConst #oldTags s))) ;
-        WriteReg tagsRegPath #newTags Retv)
-      ) else (
+        Let tagData2 : Array nTags Bool <- ConstDef ;
+        Let tagMask2 : Array nTags Bool <-
+          if hasTags r then (
+            UpdateArray ConstDef (Const ty (Bit lgNumDXlenZ) Zmod.zero) (ConstBool true)
+          ) else (
+            ConstDef
+          ) ;
+        Act (memRegionLineWrite r (STRUCT {
+          "addr"     ::= nextLineAddr addr ;
+          "data"     ::= #rotData ;
+          "dataMask" ::= #mask2 ;
+          "tag"      ::= #tagData2 ;
+          "tagMask"  ::= #tagMask2
+        })) ;
         Retv
-      )
+      ) ;
+      Retv
     ).
 
-End RegisterMemRegionActions.
+End MemRegionActions.
 
-Arguments registerMemRegionRead r lgRegBytes regs [ty] addr memSize.
-Arguments registerMemRegionWrite r lgRegBytes regs [ty] addr stVal memSize.
-
-Definition memRegionRead
-           {ty : Kind -> Type}
-           (r : MemRegion)
-           (addr : Expr ty Addr)
-           (memSize : Expr ty (Bit LgLgNumBytesFullCapSz))
-           : Action ty (memRegionTree r) FullCapWithTag :=
-  match r.(regionKind) as k return Action ty (match k with
-                                              | InternalMem init => internalMemRegionTree r init
-                                              | ExternalMem numDXlen => externalMemRegionTree r numDXlen
-                                              | RegisterMem lg regs _ _ => registerMemRegionTree r lg regs
-                                              end) FullCapWithTag with
-  | InternalMem init => internalMemRegionRead r init addr
-  | ExternalMem numDXlen => externalMemRegionRead r numDXlen addr memSize
-  | RegisterMem lg regs _ _ => registerMemRegionRead r lg regs addr memSize
-  end.
-
-Definition memRegionWrite
-           {ty : Kind -> Type}
-           (r : MemRegion)
-           (addr : Expr ty Addr)
-           (stVal : Expr ty FullCapWithTag)
-           (memSize : Expr ty (Bit LgLgNumBytesFullCapSz))
-           : Action ty (memRegionTree r) (Bit 0) :=
-  match r.(regionKind) as k return Action ty (match k with
-                                              | InternalMem init => internalMemRegionTree r init
-                                              | ExternalMem numDXlen => externalMemRegionTree r numDXlen
-                                              | RegisterMem lg regs _ _ => registerMemRegionTree r lg regs
-                                              end) (Bit 0) with
-  | InternalMem init => internalMemRegionWrite r init addr stVal memSize
-  | ExternalMem numDXlen => externalMemRegionWrite r numDXlen addr stVal memSize
-  | RegisterMem lg regs _ _ => registerMemRegionWrite r lg regs addr stVal memSize
-  end.
+Arguments memRegionRead r [ty] addr memSize.
+Arguments memRegionWrite r [ty] addr stVal memSize.
 
 (* ===========================================================================
  * 5. Composite Memory Tree & System Routing
